template-coq/theories/BasicAst.v
@@ -209,6 +209,14 @@ Inductive cast_kind : Set :=
 | RevertCast.
 Derive NoConfusion EqDec for cast_kind.
 
+Record case_info := { ci_ind : inductive; ci_npar : nat; ci_relevance : relevance }.
+Derive NoConfusion EqDec for case_info.
+
+Definition string_of_case_info ci := 
+  "(" ^ string_of_inductive ci.(ci_ind) ^ "," ^
+  string_of_nat ci.(ci_npar) ^ "," ^
+  string_of_relevance ci.(ci_relevance) ^ ")".
+
 Inductive recursivity_kind :=
   | Finite (* = inductive *)
   | CoFinite (* = coinductive *)
@@ -231,8 +239,6 @@ Record def term := mkdef {
   dtype : term;
   dbody : term; (* the body (a lambda term). Note, this may mention other (mutually-defined) names **)
   rarg  : nat  (* the index of the recursive argument, 0 for cofixpoints **) }.
-
-
 
 Arguments dname {term} _.
 Arguments dtype {term} _.
@@ -271,9 +277,6 @@ Definition mfixpoint term := list (def term).
 Definition test_def {A} (tyf bodyf : A -> bool) (d : def A) :=
   tyf d.(dtype) && bodyf d.(dbody).
 
-Definition tCaseBrsProp {A} (P : A -> Type) (l : list (nat * A)) :=
-  All (fun x => P (snd x)) l.
-
 Definition tFixProp {A} (P P' : A -> Type) (m : mfixpoint A) :=
   All (fun x : def A => P x.(dtype) * P' x.(dbody))%type m.
 
@@ -300,14 +303,38 @@ Proof.
   now rewrite !H, !H0.
 Qed.
 
-Lemma case_brs_map_spec {A B} {P : A -> Type} {l} {f g : A -> B} :
-  tCaseBrsProp P l -> (forall x, P x -> f x = g x) ->
-  map (on_snd f) l = map (on_snd g) l.
+Hint Extern 10 (_ < _)%nat => lia : all.
+Hint Extern 10 (_ <= _)%nat => lia : all.
+Hint Extern 10 (@eq nat _ _) => lia : all.
+Hint Extern 0 (_ = _) => progress f_equal : all.
+Hint Unfold on_snd snd : all.
+
+Lemma on_snd_eq_id_spec {A B} (f : B -> B) (x : A * B) :
+  f (snd x) = snd x <->
+  on_snd f x = x.
 Proof.
-  intros. red in X.
-  eapply All_map_eq. eapply All_impl; eauto. simpl; intros.
-  apply on_snd_eq_spec; eauto.
+  destruct x; simpl; unfold on_snd; simpl. split; congruence.
 Qed.
+Hint Resolve -> on_snd_eq_id_spec : all.
+Hint Resolve -> on_snd_eq_spec : all.
+
+Lemma map_def_eq_spec {A B} (f f' g g' : A -> B) (x : def A) :
+  f (dtype x) = g (dtype x) ->
+  f' (dbody x) = g' (dbody x) ->
+  map_def f f' x = map_def g g' x.
+Proof.
+  intros. unfold map_def; f_equal; auto.
+Qed.
+Hint Resolve map_def_eq_spec : all.
+
+Lemma map_def_id_spec {A} (f f' : A -> A) (x : def A) :
+  f (dtype x) = (dtype x) ->
+  f' (dbody x) = (dbody x) ->
+  map_def f f' x = x.
+Proof.
+  intros. rewrite (map_def_eq_spec _ _ id id); auto. destruct x; auto.
+Qed.
+Hint Resolve map_def_id_spec : all.
 
 Lemma tfix_map_spec {A B} {P P' : A -> Type} {l} {f f' g g' : A -> B} :
   tFixProp P P' l -> (forall x, P x -> f x = g x) ->
@@ -320,17 +347,144 @@ Proof.
   eapply map_def_spec; eauto.
 Qed.
 
+(* Parameterized by term types as they are not yet defined. *)
+Record branch {term} := mkbranch {
+  bcontext : list aname; (* Names of binders of the branch, in "context" order.
+                          Also used for lifting/substitution for the branch body. *)
+  bbody : term; (* The branch body *) }.
+  
+Arguments branch : clear implicits.
+Arguments mkbranch {_}.
+  
+Derive NoConfusion for branch.
+Global Instance branch_eq_dec term :
+  Classes.EqDec term ->
+  Classes.EqDec (branch term).
+Proof. ltac:(Equations.Prop.Tactics.eqdec_proof). Qed.
+
+Definition string_of_branch {term} (f : term -> string) (b : branch term) :=
+  "([" ^ String.concat "," (map (string_of_name ∘ binder_name) (bcontext b)) ^ "], "
+  ^ f (bbody b) ^ ")".
+
+Definition pretty_string_of_branch {term} (f : term -> string) (b : branch term) :=
+    String.concat " " (map (string_of_name ∘ binder_name) (bcontext b)) ^ " => " ^ f (bbody b).
+  
+Definition test_branch {term} (bodyf : term -> bool) (b : branch term) :=
+  bodyf b.(bbody).
+  
+Section map_branch.
+  Context {term term' : Type}.
+  Context (bbodyf : term -> term').
+
+  Definition map_branch (b : branch term) :=
+    {| bcontext := b.(bcontext);
+       bbody := bbodyf b.(bbody) |}.
+
+  Lemma map_bbody (b : branch term) :
+    bbodyf (bbody b) = bbody (map_branch b).
+  Proof. destruct b; auto. Qed.
+End map_branch.
+
+Lemma map_branch_map_branch
+      {term term' term''}
+      (f : term' -> term'')
+      (f' : term -> term')
+      (b : branch term) :
+  map_branch f (map_branch f' b) =
+  map_branch (f ∘ f') b.
+Proof.
+  destruct b; cbv.
+  f_equal.
+Qed.
+
+Lemma map_branch_id {t} x : map_branch (@id t) x = id x.
+Proof.
+  destruct x; cbv.
+  f_equal.
+Qed.
+Hint Rewrite @map_branch_id : map.
+
+Lemma map_branch_eq_spec {A B} (f g : A -> B) (x : branch A) :
+  f (bbody x) = g (bbody x) ->
+  map_branch f x = map_branch g x.
+Proof.
+  intros. unfold map_branch; f_equal; auto.
+Qed.
+Hint Resolve map_branch_eq_spec : all.
+
+Lemma map_branch_id_spec {A} (f : A -> A) (x : branch A) :
+  f (bbody x) = (bbody x) ->
+  map_branch f x = x.
+Proof.
+  intros. rewrite (map_branch_eq_spec _ id); auto. destruct x; auto.
+Qed.
+Hint Resolve map_branch_id_spec : all.
+
+Lemma map_branches_map_branches
+      {term term' term''}
+      (f : term' -> term'')
+      (f' : term -> term')
+      (l : list (branch term)) :
+  map (fun b => map_branch f (map_branch f' b)) l =
+  map (map_branch (f ∘ f')) l.
+Proof.
+  eapply map_ext => b. apply map_branch_map_branch.
+Qed.
+
+Definition map_branches {term B} (f : term -> B) l := List.map (map_branch f) l.
+
+Definition tCaseBrsProp {A} (P : A -> Type) (l : list (branch A)) :=
+  All (fun x => P (bbody x)) l.
+
+Notation map_branches_k f k brs :=
+  (List.map (fun b => map_branch (f (#|b.(bcontext)| + k)) b) brs).
+
+Notation test_branches_k test k brs :=
+  (List.forallb (fun b => test_branch (test (#|b.(bcontext)| + k)) b) brs).
+
+Lemma map_branches_k_map_branches_k
+      {term term' term''}
+      (f : nat -> term' -> term'')
+      (g : term -> term')
+      (f' : nat -> term -> term') k
+      (l : list (branch term)) :
+  map (fun b => map_branch (f #|bcontext (map_branch g b)|) (map_branch (f' k) b)) l =
+  map (fun b => map_branch (f #|bcontext b|) (map_branch (f' k) b)) l.
+Proof.
+  eapply map_ext => b. rewrite map_branch_map_branch.
+  rewrite map_branch_map_branch.
+  now apply map_branch_eq_spec.
+Qed.
+
+Lemma case_brs_map_spec {A B} {P : A -> Type} {l} {f g : A -> B} :
+  tCaseBrsProp P l -> (forall x, P x -> f x = g x) ->
+  map_branches f l = map_branches g l.
+Proof.
+  intros. red in X.
+  eapply All_map_eq. eapply All_impl; eauto. simpl; intros.
+  apply map_branch_eq_spec; eauto.
+Qed.
+
+Lemma case_brs_map_k_spec {A B} {P : A -> Type} {k l} {f g : nat -> A -> B} :
+  tCaseBrsProp P l -> (forall k x, P x -> f k x = g k x) ->
+  map_branches_k f k l = map_branches_k g k l.
+Proof.
+  intros. red in X.
+  eapply All_map_eq. eapply All_impl; eauto. simpl; intros.
+  apply map_branch_eq_spec; eauto.
+Qed.
+
 Lemma case_brs_forallb_map_spec {A B} {P : A -> Type} {p : A -> bool}
       {l} {f g : A -> B} :
   tCaseBrsProp P l ->
-  forallb (test_snd p) l ->
+  forallb (test_branch p) l ->
   (forall x, P x -> p x -> f x = g x) ->
-  map (on_snd f) l = map (on_snd g) l.
+  map (map_branch f) l = map (map_branch g) l.
 Proof.
   intros.
   eapply All_map_eq. red in X. apply forallb_All in H.
   eapply All_impl. eapply All_prod. exact X. exact H.
-  intros [] []; unfold on_snd; cbn. f_equal. now apply H0.
+  intros [] []; unfold map_branch; cbn. f_equal. now apply H0.
 Qed.
 
 Lemma tfix_forallb_map_spec {A B} {P P' : A -> Prop} {p p'} {l} {f f' g g' : A -> B} :
