template-coq/theories/AstUtils.v
@@ -40,13 +40,11 @@ Fixpoint string_of_term (t : term) :=
   | tInd i u => "Ind(" ^ string_of_inductive i ^ "," ^ string_of_universe_instance u ^ ")"
   | tConstruct i n u => "Construct(" ^ string_of_inductive i ^ "," ^ string_of_nat n ^ ","
                                     ^ string_of_universe_instance u ^ ")"
-  | tCase (ind, i, r) p t brs =>
-    "Case(" ^ string_of_inductive ind ^ ","
-            ^ string_of_nat i ^ ","
-            ^ string_of_relevance r ^ ","
+  | tCase ci p t brs =>
+    "Case(" ^ string_of_case_info ci ^ ","
             ^ string_of_predicate string_of_term p ^ ","
             ^ string_of_term t ^ ","
-            ^ string_of_list (fun b => string_of_term (snd b)) brs ^ ")"
+            ^ string_of_list (string_of_branch string_of_term) brs ^ ")"
   | tProj (ind, i, k) c =>
     "Proj(" ^ string_of_inductive ind ^ "," ^ string_of_nat i ^ "," ^ string_of_nat k ^ ","
             ^ string_of_term c ^ ")"
@@ -159,7 +157,7 @@ Fixpoint strip_casts t :=
   | tLetIn na b t b' => tLetIn na (strip_casts b) (strip_casts t) (strip_casts b')
   | tCase ind p c brs =>
     let p' := map_predicate strip_casts strip_casts p in
-    let brs' := List.map (on_snd (strip_casts)) brs in
+    let brs' := List.map (map_branch strip_casts) brs in    
     tCase ind p' (strip_casts c) brs'
   | tProj p c => tProj p (strip_casts c)
   | tFix mfix idx =>
